signature safety conclusion

src/Signatures.v
@@ -4,45 +4,89 @@ Import BinPos.
 
 Section Safety.
   Context {type : Set} {interp_type : type -> nat -> Set}
-          {trand tmessage tskey tpkey : type} {tlist : type -> type}
+          {trand tmessage tskey tpkey tbool : type} {tlist : type -> type}
           {tprod : type -> type -> type}
-          {func : type -> type -> Set}
-          {skeygen : func trand tskey} (* secret key generation (from randomness) *)
+          {func : type -> type -> Set}.
+  Context {skeygen : func trand tskey} (* secret key generation (from randomness) *)
           {pkeygen : func tskey tpkey}  (* public key generation (from secret key) *)
-          {sign : func (tprod tmessage tskey) tmessage}. 
+          {sign : func (tprod tmessage tskey) tmessage}.
   Let expr :=
     @expr type interp_type trand tmessage tlist tprod func.
 
-  Context {tmessage_eq : forall m1 m2 : expr tmessage, Prop}.
-
   Inductive signature_safe (sk : positive) :
-    forall {t}, expr t -> (expr tmessage -> Prop) -> Prop :=
+    forall {t}, expr t -> list (expr tmessage) -> Prop :=
   | sconst : forall t eta,
-      @signature_safe sk t (expr_const eta) (fun m => False)
-  | srand_eq : signature_safe sk (expr_random sk) (fun m => True)
+      @signature_safe sk t (expr_const eta) nil
   | srand_neq :
       forall i, i <> sk ->
-                signature_safe sk (expr_random i) (fun m => False)
+                signature_safe sk (expr_random i) nil
   | sadv : forall e s, signature_safe sk e s ->
                        signature_safe sk (expr_adversarial e) s
   | spkeygen :
         signature_safe sk
                        (expr_func pkeygen (expr_func skeygen (expr_random sk)))
-                       (fun m => False)
+                       nil
   | ssign :
       forall m s,
         signature_safe sk m s -> 
         signature_safe sk
                        (expr_func sign
                                   (expr_pair m (expr_func skeygen (expr_random sk))))
-                       (fun m' => tmessage_eq m m' \/ s m')
+                       (m :: s)
   | sfunc : forall {t1 t2} (f : func t1 t2) e s,
       signature_safe sk e s ->
       signature_safe sk (expr_func f e) s
   | spair : forall {t1 t2} (e1: expr t1) (e2: expr t2) s1 s2,
       signature_safe sk e1 s1 ->
       signature_safe sk e2 s2 ->
-      signature_safe sk (expr_pair e1 e2) (fun m => s1 m \/ s2 m)
+      signature_safe sk (expr_pair e1 e2) (s1 ++ s2)
   .
+
+  Context {eq_dec : EqDec.EqDec type}
+          {eq_dec_interp_type : forall (t : type) (eta : nat),
+              EqDec.EqDec (interp_type t eta)}.
+  Context {cast_rand : forall eta : nat,
+              Bvector.Bvector eta ->
+              interp_type trand eta}
+          {interp_func : forall t1 t2 : type,
+              func t1 t2 ->
+              forall eta : nat,
+                interp_type t1 eta ->
+                interp_type t2 eta}
+          {interp_pair : forall (t1 t2 : type) (eta : nat),
+              interp_type t1 eta ->
+              interp_type t2 eta ->
+              interp_type (tprod t1 t2) eta}
+          {interp_expr : forall t eta, expr t -> interp_type t eta}.
+  Let indist :=
+    @indist type eq_dec interp_type eq_dec_interp_type
+            tbool trand tmessage tlist tprod func
+            cast_rand interp_func interp_pair.
+
+  Context {tcons : forall t, func (tprod (tlist t) t) (tlist t) }.
+  Context {tnil : forall t, expr (tlist t) }.
+  Fixpoint adv_knowledge msgs : expr (tlist tmessage) :=
+    match msgs with
+    | nil => tnil _
+    | cons m msgs' =>
+      expr_func (tcons _)
+                (expr_pair (adv_knowledge msgs') m)
+    end.
+
+  Context {tand : func (tprod tbool tbool) tbool}.
+  Context {tin : forall t, func (tprod (tlist t) t) tbool}.
+  Lemma signature_safe_conclusion (sk : positive) {t} (e : expr t) S
+    (verify : func tmessage tbool) :
+    signature_safe sk e S ->
+    forall (adv : expr (tlist tmessage) -> expr tmessage),
+      let x := adv (adv_knowledge S) in
+      indist tbool
+             (expr_func verify x)
+             (expr_func tand
+                        (expr_pair
+                           (expr_func verify x)
+                           (expr_func (tin _) (expr_pair (adv_knowledge S) x)))).
+  Proof.
+  Admitted.
 
 End Safety.
